simplify AST

ExtParser/AST.lean
@@ -3,35 +3,35 @@ import ExtParser.CoreParser
 namespace AST
   open CoreParser
 
-  inductive PreAST' (n : Nat) (b : Nat) where
+  inductive PreAST (n : Nat) (b : Nat) where
     | skip (s e : Fin b) (G : PEG n)
     | ε (s e : Fin b)
     | any (s e : Fin b) (x : Char)
     | terminal (s e : Fin b) (a x : Char)
-    | nonTerminal (s e : Fin b) (A : Fin n) (T : PreAST' n b)
-    | seq (s e : Fin b) (T1 T2 : PreAST' n b)
-    | prior (s e : Fin b) (T1 T2 : PreAST' n b)
-    | star (s e : Fin b) (T0 TS : PreAST' n b)
-    | notP (s e : Fin b) (T : PreAST' n b)
+    | nonTerminal (s e : Fin b) (A : Fin n) (T : PreAST n b)
+    | seq (s e : Fin b) (T1 T2 : PreAST n b)
+    | prior (s e : Fin b) (T1 T2 : PreAST n b)
+    | star (s e : Fin b) (T0 TS : PreAST n b)
+    | notP (s e : Fin b) (T : PreAST n b)
 
-  inductive SkipPreAST' : PreAST' n b → Prop where
-    | skip : SkipPreAST' (.skip s e G)
+  inductive PreAST.SkipPreAST : PreAST n b → Prop where
+    | skip : SkipPreAST (.skip s e G)
 
-  inductive StarPreAST' : PreAST' n b → Prop where
-    | star : StarPreAST' (.star s e T0 TS)
+  inductive PreAST.StarPreAST : PreAST n b → Prop where
+    | star : StarPreAST (.star s e T0 TS)
 
-  inductive PreAST'.IsValid : PreAST' n b → Prop where
+  inductive PreAST.IsValid : PreAST n b → Prop where
     | skip : IsValid (.skip s e G)
     | ε : IsValid (.ε s e)
     | any : IsValid (.any s e x)
     | terminal : IsValid (.terminal s e a x)
-    | nonTerminal : IsValid sub_T → ¬SkipPreAST' sub_T → IsValid (.nonTerminal s e A sub_T)
-    | seq : IsValid T1 → IsValid T2 → ¬SkipPreAST' T1 → IsValid (.seq s e T1 T2)
-    | prior : IsValid T1 → IsValid T2 → ¬SkipPreAST' T1 → IsValid (.prior s e T1 T2)
-    | star : IsValid T0 → IsValid TS → ¬SkipPreAST' T0 → (SkipPreAST' TS ∨ StarPreAST' TS) → IsValid (.star s e T0 TS)
-    | notP : IsValid sub_T → ¬SkipPreAST' sub_T → IsValid (.notP s e sub_T)
+    | nonTerminal : IsValid sub_T → ¬SkipPreAST sub_T → IsValid (.nonTerminal s e A sub_T)
+    | seq : IsValid T1 → IsValid T2 → ¬SkipPreAST T1 → IsValid (.seq s e T1 T2)
+    | prior : IsValid T1 → IsValid T2 → ¬SkipPreAST T1 → IsValid (.prior s e T1 T2)
+    | star : IsValid T0 → IsValid TS → ¬SkipPreAST T0 → (SkipPreAST TS ∨ StarPreAST TS) → IsValid (.star s e T0 TS)
+    | notP : IsValid sub_T → ¬SkipPreAST sub_T → IsValid (.notP s e sub_T)
 
-  def PreAST'.size (T : PreAST' n b) : Nat :=
+  def PreAST.size (T : PreAST n b) : Nat :=
     match T with
     | .skip _ _ _ => 0
     | .ε _ _ => 0
@@ -43,7 +43,7 @@ namespace AST
     | .star _ _ T0 TS => T0.size + TS.size + 1
     | .notP _ _ T => T.size + 1
   
-  def PreAST'.start (T : PreAST' n b) : Fin b :=
+  def PreAST.start (T : PreAST n b) : Fin b :=
     match T with
     | .skip s _ _             => s
     | .ε s _                  => s
@@ -55,7 +55,7 @@ namespace AST
     | .star s _ _ _           => s
     | .notP s _ _             => s
 
-  def PreAST'.end (T : PreAST' n b) : Fin b :=
+  def PreAST.end (T : PreAST n b) : Fin b :=
     match T with
     | .skip _ e _             => e
     | .ε _ e                  => e
@@ -67,43 +67,35 @@ namespace AST
     | .star _ e _ _           => e
     | .notP _ e _             => e
 
-  structure PreAST (n : Nat) (b : Nat) where
-    T : PreAST' n b
-    valid_T : PreAST'.IsValid T
-  
-  def PreAST.start (T : PreAST n b) : Fin b := T.T.start
-  def PreAST.end (T : PreAST n b) : Fin b := T.T.end
-
   mutual
 
-  inductive SuccessAST : PreAST n b → Prop where
-    | ε : s = e → SuccessAST { T := .ε s e, valid_T := .ε }
-    | any : s.inbound_succ h = e → SuccessAST { T := .any s e x, valid_T := .any }
-    | terminal : s.inbound_succ h = e → a = x → SuccessAST { T := .terminal s e a x, valid_T := .terminal }
-    | nonTerminal : SuccessAST T → SuccessAST { T := .nonTerminal s e A T.T, valid_T := .nonTerminal T.valid_T h}
-    | seq : SuccessAST T1 → SuccessAST T2 → SuccessAST { T := .seq s e T1.T T2.T, valid_T := .seq T1.valid_T T2.valid_T h }
-    | prior_S : ∀ {T2 : PreAST n b}, SuccessAST T1 → SuccessAST { T := .prior s e T1.T T2.T, valid_T := .prior T1.valid_T T2.valid_T h }
-    | prior_FS : FailureAST T1 → SuccessAST T2 → SuccessAST { T := .prior s e T1.T T2.T, valid_T := .prior T1.valid_T T2.valid_T h }
-    | star_F : ∀ {TS : PreAST n b} {h2 : SkipPreAST' TS.T ∨ StarPreAST' TS.T}, FailureAST T0 → SuccessAST { T := .star s e T0.T TS.T, valid_T := .star T0.valid_T TS.valid_T h1 h2 }
-    | star_SS : SuccessAST T0 → SuccessAST TS → SuccessAST { T := .star s e T0.T TS.T, valid_T := .star T0.valid_T TS.valid_T h1 h2 }
-    | notP : FailureAST T → SuccessAST { T := .notP s e T.T, valid_T := .notP T.valid_T h }
+  inductive PreAST.SuccessAST : PreAST n b → Prop where
+    | ε : s = e → SuccessAST (.ε s e)
+    | any : s.inbound_succ h = e → SuccessAST (.any s e x)
+    | terminal : s.inbound_succ h = e → a = x → SuccessAST (.terminal s e a x)
+    | nonTerminal : SuccessAST T → SuccessAST (.nonTerminal s e A T)
+    | seq : SuccessAST T1 → SuccessAST T2 → SuccessAST (.seq s e T1 T2)
+    | prior_S : SuccessAST T1 → SuccessAST (.prior s e T1 T2)
+    | prior_FS : FailureAST T1 → SuccessAST T2 → SuccessAST (.prior s e T1 T2)
+    | star_F : FailureAST T0 → SuccessAST (.star s e T0 TS)
+    | star_SS : SuccessAST T0 → SuccessAST TS → SuccessAST (.star s e T0 TS)
+    | notP : FailureAST T → SuccessAST (.notP s e T)
 
-  inductive FailureAST : PreAST n b → Prop where
-    | any : s = e → FailureAST { T := .any s e x, valid_T := .any }
-    | terminal_mismatch : s.inbound_succ h = e → a ≠ x → FailureAST { T := .terminal s e a x, valid_T := .terminal }
-    | terminal_empty : s = e → FailureAST { T := .terminal s e a x, valid_T := .terminal }
-    | nonTerminal : FailureAST T → FailureAST { T := .nonTerminal s e A T.T, valid_T := .nonTerminal T.valid_T h}
-    | seq_F : ∀ {T2 : PreAST n b}, FailureAST T1 → FailureAST { T := .seq s e T1.T T2.T, valid_T := .seq T1.valid_T T2.valid_T h }
-    | seq_SF : SuccessAST T1 → FailureAST T2 → FailureAST { T := .seq s e T1.T T2.T, valid_T := .seq T1.valid_T T2.valid_T h }
-    | prior : FailureAST T1 → FailureAST T2 → FailureAST { T := .prior s e T1.T T2.T, valid_T := .prior T1.valid_T T2.valid_T h }
-    | notP : SuccessAST T → FailureAST { T := .notP s e T.T, valid_T := .notP T.valid_T h }
+  inductive PreAST.FailureAST : PreAST n b → Prop where
+    | any : s = e → FailureAST (.any s e x)
+    | terminal_mismatch : s.inbound_succ h = e → a ≠ x → FailureAST (.terminal s e a x)
+    | terminal_empty : s = e → FailureAST (.terminal s e a x)
+    | nonTerminal : FailureAST T → FailureAST (.nonTerminal s e A T)
+    | seq_F : FailureAST T1 → FailureAST (.seq s e T1 T2)
+    | seq_SF : SuccessAST T1 → FailureAST T2 → FailureAST (.seq s e T1 T2)
+    | prior : FailureAST T1 → FailureAST T2 → FailureAST (.prior s e T1 T2)
+    | notP : SuccessAST T → FailureAST (.notP s e T)
 
   end
 
-  theorem SuccessAST.ne_failure : ∀ {T : PreAST n b}, SuccessAST T → ¬FailureAST T := by
-    intro T hs hf;
+  theorem PreAST.SuccessAST.ne_failure : ∀ {T : PreAST n b}, PreAST.IsValid T → SuccessAST T → ¬FailureAST T := by
+    intro T valid_T hs hf;
     match T with
-    | .mk T valid_T => match T with
       | .skip _ _ _ => cases hs;
       | .ε _ _ => cases hf;
       | .any _ _ _ => cases hs; cases hf; apply absurd (by assumption); apply Fin.ne_of_val_ne; apply Nat.ne_of_lt; apply Fin.lt_from_inbound_succ; assumption;
@@ -111,261 +103,141 @@ namespace AST
       | .nonTerminal s e A _ => match hs with
         | .nonTerminal (T := Ts) st =>
           {
-            match Ts with
-            | .mk Ts' _ => simp at hf; match hf with
-              | .nonTerminal (T := Ts) ft => 
-                {
-                  have _ : PreAST'.size Ts.T < PreAST'.size (PreAST'.nonTerminal s e A Ts.T) := by
-                  {
-                    rw [PreAST'.size]; apply Nat.lt_succ_self;
-                  }
-                  apply absurd ft; apply ne_failure; exact st;
-                }
+            match hf with
+            | .nonTerminal (T := Ts) ft => 
+              {
+                apply absurd ft; apply ne_failure; cases valid_T; assumption; assumption;
+              }
           }
       | .seq s e _ _ => match hs with
         | .seq (T1 := T1) (T2 := T2) st1 st2 =>
           {
-            match T1, T2 with
-            | .mk T1' _, .mk T2' _ => simp at hf; match hf with
+            match hf with
               | .seq_F (T1 := T1) (T2 := T2) ft1 =>
                 {
-                  have _ : PreAST'.size T1.T < PreAST'.size (PreAST'.seq s e T1.T T2.T) := by
-                  {
-                    rw [PreAST'.size];
-                    apply Nat.lt_succ_of_le; simp;
-                    apply Nat.le_add_right;
-                  }
-                  apply absurd ft1; apply ne_failure; exact st1;
+                  apply absurd ft1; apply ne_failure; cases valid_T; assumption; assumption;
                 }
               | .seq_SF (T1 := T1) (T2 := T2) _ ft2 =>
                 {
-                  have _ : PreAST'.size T2.T < PreAST'.size (PreAST'.seq s e T1.T T2.T) := by
-                  {
-                    rw [PreAST'.size];
-                    apply Nat.lt_succ_of_le; simp;
-                    apply Nat.le_add_left;
-                  }
-                  apply absurd ft2; apply ne_failure; exact st2;
+                  apply absurd ft2; apply ne_failure; cases valid_T; assumption; assumption;
                 }
           }
       | .prior s e _ _ => match hf with
         | .prior (T1 := T1) (T2 := T2) ft1 ft2 =>
           {
-            match T1, T2 with
-            | .mk T1' _, .mk T2' _ => simp at hs; match hs with
+            match hs with
               | .prior_S (T1 := T1) (T2 := T2) st1 =>
                 {
-                  have _ : PreAST'.size T1.T < PreAST'.size (PreAST'.prior s e T1.T T2.T) := by
-                  {
-                    rw [PreAST'.size];
-                    apply Nat.lt_succ_of_le; simp;
-                    apply Nat.le_add_right;
-                  }
-                  apply absurd ft1; apply ne_failure; exact st1;
+                  apply absurd ft1; apply ne_failure; cases valid_T; assumption; assumption;
                 }
               | .prior_FS (T1 := T1) (T2 := T2) _ st2 =>
                 {
-                  have _ : PreAST'.size T2.T < PreAST'.size (PreAST'.prior s e T1.T T2.T) := by
-                  {
-                    rw [PreAST'.size];
-                    apply Nat.lt_succ_of_le; simp;
-                    apply Nat.le_add_left;
-                  }
-                  apply absurd ft2; apply ne_failure; exact st2;
+                  apply absurd ft2; apply ne_failure; cases valid_T; assumption; assumption;
                 }
           }
       | .star s e _ _ => cases hf;
       | .notP s e _ => match hs with
         | .notP (T := T) ft =>
           {
-            match T with
-            | .mk T' _ => simp at hf; match hf with
+            match hf with
               | .notP (T := T) st =>
                 {
-                  have _ : PreAST'.size T.T < PreAST'.size (PreAST'.notP s e T.T) := by
-                  {
-                    rw [PreAST'.size];
-                    apply Nat.lt_succ_of_le; simp;
-                  }
-                  apply absurd ft; apply ne_failure; exact st;
+                  apply absurd ft; apply ne_failure; cases valid_T; assumption; assumption;
                 }
           }
-  termination_by SuccessAST.ne_failure T _ _ => T.T.size
 
-  theorem FailureAST.ne_success : ∀ {T : PreAST n b}, FailureAST T → ¬SuccessAST T := by
-    intro T hf hs;
-    exact SuccessAST.ne_failure hs hf;
+  theorem PreAST.FailureAST.ne_success : ∀ {T : PreAST n b}, PreAST.IsValid T → FailureAST T → ¬SuccessAST T := by
+    intro T valid_T hf hs;
+    exact SuccessAST.ne_failure valid_T hs hf;
 
-  inductive TypeAST : PreAST n b → Prop
-    | success : SuccessAST T → TypeAST T
-    | failure : FailureAST T → TypeAST T
-    | undefined : ¬SuccessAST T → ¬FailureAST T → TypeAST T
-  
-  def PreAST.check_type (T : PreAST n b) : TypeAST T :=
-    match T with
-    | .mk T valid_T => match T with
-      | .skip s e G => .undefined (by intro h; cases h;) (by intro h; cases h;)
-      | .ε s e => match decEq s e with
-        | isTrue heq => .success (.ε heq)
-        | isFalse hne => .undefined (by intro h; cases h; contradiction) (by intro h; cases h;)
-      | .any s e x => match decEq s e, decEq s.val.succ b with
-        | isTrue heq_e, _ => .failure (.any heq_e)
-        | isFalse hne_e, isTrue heq_b => .undefined (by intro h; cases h; contradiction;) (by intro h; cases h; contradiction)
-        | isFalse hne_e, isFalse hne_b => match decEq (s.inbound_succ hne_b) e with
-          | isTrue g => .success (.any g)
-          | isFalse g => .undefined (by intro h; cases h; apply absurd _ g; simp [Fin.inbound_succ] at *; apply Fin.eq_of_val_eq; apply Fin.val_eq_of_eq; assumption) (by intro h; cases h; contradiction;)
-      | .terminal s e a x => match decEq s e, decEq s.val.succ b, decEq a x with
-        | isTrue heq_e, _, _ => .failure (.terminal_empty heq_e)
-        | isFalse hne_e, isTrue heq_b, _ => .undefined (by intro h; cases h; contradiction;) (by intro h; cases h; contradiction; contradiction;)
-        | isFalse hne_e, isFalse hne_b, isTrue heq_ax => match decEq (s.inbound_succ hne_b) e with
-          | isTrue g => .success (.terminal g heq_ax)
-          | isFalse g => .undefined (by intro h; cases h; apply absurd _ g; simp [Fin.inbound_succ] at *; apply Fin.eq_of_val_eq; apply Fin.val_eq_of_eq; assumption) (by intro h; cases h; contradiction; contradiction;)
-        | isFalse hne_e, isFalse hne_b, isFalse hne_ax => match decEq (s.inbound_succ hne_b) e with
-          | isTrue g => .failure (.terminal_mismatch g hne_ax)
-          | isFalse g => .undefined (by intro h; cases h; contradiction;) (by intro h; cases h; apply absurd _ g; simp [Fin.inbound_succ] at *; apply Fin.eq_of_val_eq; apply Fin.val_eq_of_eq; assumption; contradiction;)
-      | .nonTerminal s e A sub_T => match valid_T with
-        | .nonTerminal wf ns =>
-          let T_ast : PreAST n b := (PreAST.mk sub_T wf);
-          have g : (¬SkipPreAST' T_ast.T) := by simp; exact ns;
-          match check_type T_ast with
-          | .success h => .success (.nonTerminal (h := g) h)
-          | .failure h => .failure (.nonTerminal (h := g) h)
-          | .undefined hs hf => .undefined (by intro h; cases h; contradiction;) (by intro h; cases h; contradiction;)
-      | .seq s e T1 T2 => match valid_T with
-        | .seq wf1 wf2 ns =>
-          let T1_ast : PreAST n b := (PreAST.mk T1 wf1);
-          let T2_ast : PreAST n b := (PreAST.mk T2 wf2);
-          have g : (¬SkipPreAST' T1_ast.T) := by simp; exact ns;
-          match check_type T1_ast, check_type T2_ast with
-          | .undefined h1s h1f, _ => .undefined (by intro h; cases h; contradiction;) (by intro h; cases h; contradiction; contradiction;)
-          | .success h1, .success h2 => .success (.seq (h := g) h1 h2)
-          | .success h1, .failure h2 => .failure (.seq_SF (h := g) h1 h2)
-          | .success h1, .undefined h2s h2f => .undefined (by intro h; cases h; contradiction;) (by intro h; cases h; {apply absurd _ (h1.ne_failure); assumption}; {apply absurd _ h2f; assumption})
-          | .failure h1, _ => .failure (.seq_F (T2 := T2_ast) (h := g) h1)
-      | .prior s e T1 T2 => match valid_T with
-        | .prior wf1 wf2 ns =>
-          let T1_ast : PreAST n b := (PreAST.mk T1 wf1);
-          let T2_ast : PreAST n b := (PreAST.mk T2 wf2);
-          have g : (¬SkipPreAST' T1_ast.T) := by simp; exact ns;
-          match check_type T1_ast, check_type T2_ast with
-          | .undefined h1s h1f, _ => .undefined (by intro h; cases h; contradiction; contradiction;) (by intro h; cases h; contradiction;)
-          | .success h1, _ => .success (.prior_S (T2 := T2_ast) (h := g) h1)
-          | .failure h1, .success h2 => .success (.prior_FS (h := g) h1 h2)
-          | .failure h1, .failure h2 => .failure (.prior (h := g) h1 h2)
-          | .failure h1, .undefined h2s h2f => .undefined (by intro h; cases h; apply absurd _ (h1.ne_success); assumption; apply absurd _ h2s; assumption) (by intro h; cases h; apply absurd _ h2f; assumption)
-      | .star s e T0 TS => match valid_T with
-        | .star wf0 wfS n0 nS =>
-          let T0_ast : PreAST n b := (PreAST.mk T0 wf0);
-          let TS_ast : PreAST n b := (PreAST.mk TS wfS);
-          have g1 : (¬SkipPreAST' T0_ast.T) := by simp; exact n0;
-          have g2 : SkipPreAST' TS_ast.T ∨ StarPreAST' TS_ast.T := by 
-          {
-            cases nS; simp; apply Or.inl; assumption; simp; apply Or.inr; assumption;
-          }
-          match check_type T0_ast, check_type TS_ast with
-          | .undefined h1s h1f, _ => .undefined (by intro h; cases h; apply absurd _ h1f; assumption; apply absurd _ h1s; assumption) (by intro h; cases h;)
-          | .failure h0, _ => .success (.star_F (TS := TS_ast) (h1 := g1) (h2 := g2) h0)
-          | .success h0, .success hs => .success (.star_SS (TS := TS_ast) (h1 := g1) (h2 := g2) h0 hs)
-          | .success h0, .failure hs => .undefined (by intro h; cases h; apply absurd _ h0.ne_failure; assumption; apply absurd _ hs.ne_success; assumption) (by intro h; cases h;)
-          | .success h0, .undefined h2s h2f => .undefined (by intro h; cases h; apply absurd _ h0.ne_failure; assumption; contradiction) (by intro h; cases h;)
-      | .notP s e sub_T => match valid_T with
-        | .notP wf ns =>
-          let T_ast : PreAST n b := (PreAST.mk sub_T wf);
-          have g : (¬SkipPreAST' T_ast.T) := by simp; exact ns;
-          match check_type T_ast with
-          | .success h => .failure (.notP (h := g) h)
-          | .failure h => .success (.notP (h := g) h)
-          | .undefined hs hf => .undefined (by intro h; cases h; contradiction) (by intro h; cases h; contradiction)
-
-  theorem PreAST.star_cannot_fail : ∀ {T : PreAST n b}, StarPreAST' T.T → ¬FailureAST T := by
+  theorem PreAST.PreAST.star_cannot_fail : ∀ {T : PreAST n b}, StarPreAST T → ¬FailureAST T := by
     intro T h_star h_fail;
-    match T with
-    | .mk T valid_T => simp_all; cases h_star; cases h_fail
+    cases h_star; cases h_fail;
   
   def PreAST.IsMeaningful (T : PreAST n b) : Prop := SuccessAST T ∨ FailureAST T
 
   inductive PreAST.IsWellformed : PreAST n b → Prop where
-    | ε :           IsMeaningful (mk (.ε s e) h) 
-                    → IsWellformed (mk (.ε s e) h)
-    | any :         IsMeaningful (mk (.any s e x) h) 
-                    → IsWellformed (mk (.any s e x) h)
-    | terminal :    IsMeaningful (mk (.terminal s e a x) h) 
-                    → IsWellformed (mk (.terminal s e a x) h)
-    | nonTerminal : ∀ {sub_T : PreAST n b} {h : PreAST'.IsValid (PreAST'.nonTerminal s e A sub_T.T)},
+    | ε :           IsMeaningful (.ε (n := n) (b := b) s e)
+                    → IsWellformed (.ε (n := n) (b := b) s e)
+    | any :         IsMeaningful (.any (n := n) (b := b) s e x)
+                    → IsWellformed (.any (n := n) (b := b) s e x)
+    | terminal :    IsMeaningful (.terminal (n := n) (b := b) s e a x)
+                    → IsWellformed (.terminal (n := n) (b := b) s e a x)
+    | nonTerminal : ∀ {sub_T : PreAST n b},
                     s = sub_T.start → e = sub_T.end 
                     → IsWellformed sub_T 
-                    → IsWellformed (mk (.nonTerminal s e A sub_T.T) h)
-    | seq_F :       ∀ {T1 T2 : PreAST n b} {h : PreAST'.IsValid (PreAST'.seq s e T1.T T2.T)},
+                    → IsWellformed (.nonTerminal s e A sub_T)
+    | seq_F :       ∀ {T1 T2 : PreAST n b},
                     s = T1.start → T1.end = T2.start → e = T2.end → T2.start = T2.end
-                    → IsWellformed T1 → FailureAST T1 → SkipPreAST' T2.T
-                    → IsWellformed (mk (.seq s e T1.T T2.T) h)
-    | seq_S :       ∀ {T1 T2 : PreAST n b} {h : PreAST'.IsValid (PreAST'.seq s e T1.T T2.T)},
+                    → IsWellformed T1 → FailureAST T1 → SkipPreAST T2
+                    → IsWellformed (.seq s e T1 T2)
+    | seq_S :       ∀ {T1 T2 : PreAST n b},
                     s = T1.start → T1.end = T2.start → e = T2.end 
                     → IsWellformed T1 → SuccessAST T1 → IsWellformed T2
-                    → IsWellformed (mk (.seq s e T1.T T2.T) h)
-    | prior_S :     ∀ {T1 T2 : PreAST n b} {h : PreAST'.IsValid (PreAST'.prior s e T1.T T2.T)},
+                    → IsWellformed (.seq s e T1 T2)
+    | prior_S :     ∀ {T1 T2 : PreAST n b},
                     s = T1.start → s = T2.start → s = T2.end → e = T1.end 
-                    → IsWellformed T1 → SuccessAST T1 → SkipPreAST' T2.T
-                    → IsWellformed (mk (.prior s e T1.T T2.T) h)
-    | prior_F :     ∀ {T1 T2 : PreAST n b} {h : PreAST'.IsValid (PreAST'.prior s e T1.T T2.T)},
+                    → IsWellformed T1 → SuccessAST T1 → SkipPreAST T2
+                    → IsWellformed (.prior s e T1 T2)
+    | prior_F :     ∀ {T1 T2 : PreAST n b},
                     s = T1.start → s = T2.start → e = T2.end 
                     → IsWellformed T1 → FailureAST T1 → IsWellformed T2
-                    → IsWellformed (mk (.prior s e T1.T T2.T) h)
-    | star_S :      ∀ {T0 TS : PreAST n b} {h : PreAST'.IsValid (PreAST'.star s e T0.T TS.T)},
+                    → IsWellformed (.prior s e T1 T2)
+    | star_S :      ∀ {T0 TS : PreAST n b},
                     s = T0.start → T0.end = TS.start → e = TS.end
                     → IsWellformed T0 → SuccessAST T0 → IsWellformed TS
-                    → IsWellformed (mk (.star s e T0.T TS.T) h)
-    | star_F :      ∀ {T0 TS : PreAST n b} {h : PreAST'.IsValid (PreAST'.star s e T0.T TS.T)},
+                    → IsWellformed (.star s e T0 TS)
+    | star_F :      ∀ {T0 TS : PreAST n b},
                     s = T0.start → T0.end = TS.start → TS.start = TS.end → s = e
-                    → IsWellformed T0 → FailureAST T0 → SkipPreAST' TS.T  
-                    → IsWellformed (mk (.star s e T0.T TS.T) h)
-    | notP :        ∀ {sub_T : PreAST n b} {h : PreAST'.IsValid (PreAST'.notP s e sub_T.T)},
+                    → IsWellformed T0 → FailureAST T0 → SkipPreAST TS
+                    → IsWellformed (.star s e T0 TS)
+    | notP :        ∀ {sub_T : PreAST n b},
                     s = e → s = sub_T.start
                     → IsWellformed sub_T 
-                    → IsWellformed (mk (.notP s e sub_T.T) h)
+                    → IsWellformed (.notP s e sub_T)
 
-  theorem PreAST.skip_is_not_wellformed : ∀ {T : PreAST n b}, SkipPreAST' T.T → ¬IsWellformed T := by
-    intro T h_skip hwf;
-    cases T; simp_all; cases h_skip; cases hwf;
+  theorem PreAST.skip_is_not_wellformed : ∀ {T : PreAST n b}, SkipPreAST T → ¬IsWellformed T := by
+    intro T hskip hwf;
+    cases hskip; cases hwf;
 
-  theorem PreAST.wellformed_implies_meaningful : ∀ {T : PreAST n b}, IsWellformed T → IsMeaningful T := by
-    intro T hwf;
+  theorem PreAST.valid_and_wellformed_implies_meaningful : ∀ {T : PreAST n b}, IsValid T → IsWellformed T → IsMeaningful T := by
+    intro T h_valid hwf;
     match hwf with
-    | .ε _ => assumption
-    | .any _ => assumption
-    | .terminal _ => assumption
-    | .nonTerminal (h := h_valid) _ _ hwfT =>
+    | .ε _ => assumption;
+    | .any _ => assumption;
+    | .terminal _ => assumption;
+    | .nonTerminal _ _ hwfT =>
       {
-        cases h_valid; cases wellformed_implies_meaningful hwfT;
+        cases h_valid; cases valid_and_wellformed_implies_meaningful (by assumption) hwfT;
         apply Or.inl; constructor <;> assumption;
         apply Or.inr; constructor <;> assumption;
       }
-    | .seq_F (h := h_valid) _ _ _ _ _ hf1 hskip2 =>
+    | .seq_F _ _ _ _ _ hf1 hskip2 =>
       {
         cases h_valid; apply Or.inr;
         apply FailureAST.seq_F <;> assumption;
       }
-    | .seq_S (h := h_valid) _ _ _ _ hs1 hwf2 =>
+    | .seq_S _ _ _ _ hs1 hwf2 =>
       {
-        cases h_valid; cases wellformed_implies_meaningful hwf2;
+        cases h_valid; cases valid_and_wellformed_implies_meaningful (by assumption) hwf2;
         apply Or.inl; constructor <;> assumption;
         apply Or.inr; apply FailureAST.seq_SF <;> assumption;
       }
-    | .prior_S (h := h_valid) _ _ _ _ _ hs1 hskip2 =>
+    | .prior_S _ _ _ _ _ hs1 hskip2 =>
       {
         cases h_valid; apply Or.inl;
         apply SuccessAST.prior_S <;> assumption;
       }
-    | .prior_F (h := h_valid) _ _ _ _ hf1 hwf2 =>
+    | .prior_F _ _ _ _ hf1 hwf2 =>
       {
-        cases h_valid; cases wellformed_implies_meaningful hwf2;
+        cases h_valid; cases valid_and_wellformed_implies_meaningful (by assumption) hwf2;
         apply Or.inl; apply SuccessAST.prior_FS <;> assumption;
         apply Or.inr; constructor <;> assumption;
       }
-    | .star_S (TS := TS) (h := h_valid) _ _ _ _ hs0 hwfS =>
+    | .star_S (TS := TS) _ _ _ _ hs0 hwfS =>
       {
         match h_valid with
-        | PreAST'.IsValid.star _ _ _ svs => 
+        | PreAST.IsValid.star _ _ _ svs => 
           match svs with
           | Or.inl hskip =>
             {
@@ -375,105 +247,115 @@ namespace AST
           | Or.inr hstar =>
             {
               apply Or.inl; apply SuccessAST.star_SS;
-              assumption; apply Or.inr; assumption; assumption;
-              match wellformed_implies_meaningful hwfS with
+              assumption;
+              match valid_and_wellformed_implies_meaningful (by assumption) hwfS with
               | Or.inl _ => assumption
-              | Or.inr hf => cases TS; cases hstar; cases hf;
+              | Or.inr hf => cases hstar; cases hf;
             }
         
       }
-    | .star_F (h := h_valid) _ _ _ _ _ hf0 hskipS =>
+    | .star_F _ _ _ _ _ hf0 hskipS =>
       {
         cases h_valid; apply Or.inl;
         apply SuccessAST.star_F <;> assumption;
       }
-    | .notP (h := h_valid) _ _ hwfT =>
+    | .notP _ _ hwfT =>
       {
-        cases h_valid; cases wellformed_implies_meaningful hwfT;
+        cases h_valid; cases valid_and_wellformed_implies_meaningful (by assumption) hwfT;
         apply Or.inr; constructor <;> assumption;
         apply Or.inl; constructor <;> assumption;
       }
   
-  theorem PreAST.start_le_end : ∀ {T : PreAST n b}, IsWellformed T → T.start ≤ T.end := by
-    intro T hwf;
+  theorem PreAST.valid_and_wellformed_implies_start_le_end : ∀ {T : PreAST n b}, IsValid T → IsWellformed T → T.start ≤ T.end := by
+    intro T h_valid hwf;
     match hwf with
     | .ε hm =>
       {
-        cases T; simp [PreAST.start, PreAST.end, PreAST'.start, PreAST'.end];
+        simp [PreAST.start, PreAST.end, PreAST.start, PreAST.end];
         match hm with
         | Or.inl hs => cases hs; apply Nat.le_of_eq; apply Fin.val_eq_of_eq; assumption;
       }
     | .any hm =>
       {
-        cases T; simp [PreAST.start, PreAST.end, PreAST'.start, PreAST'.end];
+        simp [PreAST.start, PreAST.end, PreAST.start, PreAST.end];
         match hm with
         | Or.inl hs => cases hs; apply Nat.le_of_lt; apply Fin.lt_from_inbound_succ; assumption;
         | Or.inr hf => cases hf; apply Nat.le_of_eq; apply Fin.val_eq_of_eq; assumption;
       }
     | .terminal hm =>
       {
-        cases T; simp [PreAST.start, PreAST.end, PreAST'.start, PreAST'.end];
+        simp [PreAST.start, PreAST.end, PreAST.start, PreAST.end];
         match hm with
         | Or.inl hs => cases hs; apply Nat.le_of_lt; apply Fin.lt_from_inbound_succ; assumption;
         | Or.inr hf => cases hf; apply Nat.le_of_lt; apply Fin.lt_from_inbound_succ; assumption; apply Nat.le_of_eq; apply Fin.val_eq_of_eq; assumption;
       }
-    | .nonTerminal (h := h_valid) hssT heeT hwfT =>
+    | .nonTerminal hssT heeT hwfT =>
       {
-        cases T; simp [PreAST.start, PreAST.end, PreAST'.start, PreAST'.end];
+        cases h_valid; simp [PreAST.start, PreAST.end, PreAST.start, PreAST.end];
         rw [hssT, heeT];
-        apply start_le_end;
-        assumption;
+        apply valid_and_wellformed_implies_start_le_end <;> assumption;
       }
-    | .seq_F (h := h_valid) hss1 he1s2 hee2 hs2e2 hwf1 _ hskip2 =>
+    | .seq_F hss1 he1s2 hee2 hs2e2 hwf1 _ hskip2 =>
       {
-        cases T; simp [PreAST.start, PreAST.end, PreAST'.start, PreAST'.end];
+        cases h_valid; simp [PreAST.start, PreAST.end, PreAST.start, PreAST.end];
         rw [hss1, hee2, ←hs2e2, ←he1s2]
-        apply start_le_end hwf1;
+        apply valid_and_wellformed_implies_start_le_end <;> assumption;
       }
-    | .seq_S (h := h_valid) hss1 he1s2 hee2 hwf1 _ hwf2 =>
+    | .seq_S hss1 he1s2 hee2 hwf1 _ hwf2 =>
       {
-        cases T; simp [PreAST.start, PreAST.end, PreAST'.start, PreAST'.end];
+        cases h_valid; simp [PreAST.start, PreAST.end, PreAST.start, PreAST.end];
         rw [hss1, hee2];
         apply Nat.le_trans;
-        apply start_le_end hwf1;
+        apply valid_and_wellformed_implies_start_le_end (by assumption) hwf1;
         rw [he1s2];
-        apply start_le_end hwf2;
+        apply valid_and_wellformed_implies_start_le_end (by assumption) hwf2;
       }
-    | .prior_S (h := h_valid) hss1 _ _ hee1 hwf1 _ hskip2 =>
+    | .prior_S hss1 _ _ hee1 hwf1 _ hskip2 =>
       {
-        cases T; simp [PreAST.start, PreAST.end, PreAST'.start, PreAST'.end];
+        cases h_valid; simp [PreAST.start, PreAST.end, PreAST.start, PreAST.end];
         rw [hss1, hee1];
-        apply start_le_end hwf1;
+        apply valid_and_wellformed_implies_start_le_end (by assumption) hwf1;
       }
-    | .prior_F (h := h_valid) _ hss2 hee2 _ _ hwf2 =>
+    | .prior_F _ hss2 hee2 _ _ hwf2 =>
       {
-        cases T; simp [PreAST.start, PreAST.end, PreAST'.start, PreAST'.end];
+        cases h_valid; simp [PreAST.start, PreAST.end, PreAST.start, PreAST.end];
         rw [hss2, hee2];
-        apply start_le_end hwf2;
+        apply valid_and_wellformed_implies_start_le_end (by assumption) hwf2;
       }
-    | .star_S (TS := TS) (h := h_valid) hss0 he0sS heeS hwf0 _ hwfS =>
+    | .star_S (TS := TS) hss0 he0sS heeS hwf0 _ hwfS =>
       {
-        cases T; simp [PreAST.start, PreAST.end, PreAST'.start, PreAST'.end];
+        cases h_valid; simp [PreAST.start, PreAST.end, PreAST.start, PreAST.end];
         rw [hss0, heeS];
         apply Nat.le_trans;
-        apply start_le_end hwf0;
+        apply valid_and_wellformed_implies_start_le_end (by assumption) hwf0;
         rw [he0sS];
-        apply start_le_end hwfS;
+        apply valid_and_wellformed_implies_start_le_end (by assumption) hwfS;
       }
-    | .star_F (h := h_valid) _ _ _ hse _ _ hskipS =>
+    | .star_F _ _ _ hse _ _ hskipS =>
       {
-        cases T; simp [PreAST.start, PreAST.end, PreAST'.start, PreAST'.end];
+        cases h_valid; simp [PreAST.start, PreAST.end, PreAST.start, PreAST.end];
         rw [hse];
         apply Nat.le_refl;
       }
-    | .notP (h := h_valid) hse _ hwfT =>
+    | .notP hse _ hwfT =>
       {
-        cases T; simp [PreAST.start, PreAST.end, PreAST'.start, PreAST'.end];
+        cases h_valid; simp [PreAST.start, PreAST.end, PreAST.start, PreAST.end];
         rw [hse];
         apply Nat.le_refl;
       }
 
   structure AST (n : Nat) (b : Nat) where
     T : PreAST n b
+    valid_T : PreAST.IsValid T
     wf_T : PreAST.IsWellformed T
+  
+  def AST.size (T : AST n b) : Nat := T.T.size
+  def AST.start (T : AST n b) : Fin b := T.T.start
+  def AST.end (T : AST n b) : Fin b := T.T.end
+
+  theorem AST.meaningful (T : AST n b) : PreAST.IsMeaningful T.T := PreAST.valid_and_wellformed_implies_meaningful T.valid_T T.wf_T
+  theorem AST.start_le_end (T : AST n b) : T.start ≤ T.end := by
+    rw [AST.start, AST.end];
+    apply PreAST.valid_and_wellformed_implies_start_le_end T.valid_T T.wf_T;
+
 end AST
